icing/CakeMLtoFloVerProofsScript.sml
@@ -10,6 +10,187 @@ open preamble;
 
 val _ = new_theory "CakeMLtoFloVerProofs";
 
+Theorem isFloVerExps_toFloVerExp_succeeds:
+  ∀ es.
+    isFloVerExps es ⇒
+    ∀ e. MEM e es ⇒
+      ∀ ids freshId.
+        ∃ ids2 freshId2 fexp.
+        toFloVerExp ids freshId e = SOME (ids2, freshId2, fexp)
+Proof
+  ho_match_mp_tac isFloVerExps_ind
+  \\ rpt strip_tac \\ rfs [] \\ rveq \\ TRY (fs[isFloVerExps_def]\\NO_TAC)
+  >- (fs[isFloVerExps_def, toFloVerExp_def, lookupCMLVar_def]
+      \\ rpt (TOP_CASE_TAC \\ fs[]))
+  \\ Cases_on ‘op’ \\ fs[isFloVerExps_def, quantHeuristicsTheory.LIST_LENGTH_3]
+  \\ rveq \\ fs[]
+  >- (
+    Cases_on ‘f’ \\ fs[] \\ rveq \\ fs[]
+    \\ simp[toFloVerExp_def]
+    \\ first_x_assum (qspecl_then [‘ids’,‘freshId’] assume_tac) \\ fs[])
+  >- (
+     simp[toFloVerExp_def]
+     \\ first_assum (qspec_then ‘e1’ assume_tac)
+     \\ first_x_assum (qspec_then ‘e2’ assume_tac)
+     \\ fs[]
+     \\ last_x_assum (qspecl_then [‘ids’, ‘freshId’] assume_tac) \\ fs[]
+     \\ last_x_assum (qspecl_then [‘ids2’, ‘freshId2’] assume_tac) \\ fs[])
+  \\ simp[toFloVerExp_def]
+  \\ first_assum (qspec_then ‘e1’ assume_tac)
+  \\ first_assum (qspec_then ‘e2’ assume_tac)
+  \\ first_x_assum (qspec_then ‘e3’ assume_tac)
+  \\ fs[]
+  \\ last_x_assum (qspecl_then [‘ids’, ‘freshId’] assume_tac) \\ fs[]
+  \\ last_x_assum (qspecl_then [‘ids2’, ‘freshId2’] assume_tac) \\ fs[]
+  \\ rename1 ‘toFloVerExp ids2 freshId2 e2 = SOME (ids3, freshId3, fexp2)’
+  \\ last_x_assum (qspecl_then [‘ids3’, ‘freshId3’] assume_tac) \\ fs[]
+QED
+
+Theorem isFloVerCmd_toFloVerCmd_succeeds:
+  ∀ e ids freshId.
+    isFloVerCmd e ⇒
+    ∃ ids2 f.
+      toFloVerCmd ids freshId e = SOME (ids2, f)
+Proof
+  ho_match_mp_tac isFloVerCmd_ind
+  \\ rpt strip_tac \\ fs[isFloVerCmd_def, toFloVerCmd_def]
+  >- (
+   Cases_on ‘so’ \\ fs[lookupCMLVar_def, updateTheory.FIND_def]
+   \\ drule isFloVerExps_toFloVerExp_succeeds \\ fs[]
+   \\ disch_then (qspecl_then [‘ids’, ‘freshId’] assume_tac) \\ fs[]
+   \\ first_x_assum (qspecl_then [‘appendCMLVar (Short x) freshId2 ids2’, ‘freshId2 + 1’] assume_tac)
+   \\ fs[])
+  >- (
+   drule isFloVerExps_toFloVerExp_succeeds
+    \\ disch_then (qspecl_then [‘App op exps’,‘ids’, ‘freshId’] assume_tac) \\ fs[])
+  \\ fs[toFloVerExp_def]
+  \\ Cases_on ‘lookupCMLVar x ids’ \\ fs[]
+  \\ Cases_on ‘x'’ \\ fs[]
+QED
+
+(*
+Theorem CakeML_Flover_real_imp:
+  ∀ e ids f env st r st2.
+  isFloVerCmd e ∧
+  toFloVerCmd [] 0 e = SOME(ids, f) ∧
+  evaluate st env [toRealExp e] = (st2, Rval [Real r]) ⇒
+  bstep f (toFloVerEnv env ids) (λ e. SOME REAL) r REAL
+Proof
+  ho_match_mp_tac terminationTheory.evaluate_ind
+QED
+
+local
+  val bstep_goal =
+  “(λ f E Gamma r t.
+    ∀ e ids st env st2.
+    bstep f E Gamma r t ∧
+    E = (toFloVerEnv env ids) ∧
+    Gamma = (λ e. SOME REAL) ∧
+    t = REAL ∧
+    isFloVerCmd e ∧
+    toFloVerCmd [] 0 e = SOME(ids, f) ⇒
+    evaluate st env [toRealExp e] = (st2, Rval [Real r]))”
+in
+Theorem Flover_CakeML_real_imp:
+  ∀ f E Gamma r t.
+   (^bstep_goal) f E Gamma r t
+Proof
+
+Theorem FloVerExp_CakeML_real_imp:
+  ∀ es f r ids ids2 freshId freshId2 st env.
+  isFloVerExps es ⇒
+  ∀ e. MEM e es ∧
+  eval_expr (toFloVerEnv env ids) (λ e. SOME REAL) f r REAL ∧
+  st.fp_state.real_sem ∧
+  toFloVerExp ids freshId e = SOME(ids2, freshId2, f) ⇒
+  ∃ st2.
+  evaluate st env [toRealExp e] = (st2, Rval [Real r])
+Proof
+  ho_match_mp_tac isFloVerExps_ind \\ rpt strip_tac \\ TRY (fs[isFloVerExps_def] \\ NO_TAC)
+  >- (
+   fs[isFloVerExps_def] \\ rveq \\ fs[toFloVerExp_def]
+   \\ Cases_on  ‘∃ v y. lookupCMLVar x ids = SOME (v,y)’ \\ fs[] \\ fs[] \\ rveq
+   >- (
+    fs[toRealExp_def, terminationTheory.evaluate_def, toFloVerEnv_def,
+       ExpressionSemanticsTheory.eval_expr_cases, lookupFloVerVar_def,
+       lookupCMLVar_def]
+    \\ ‘FIND (λ (m,i). y = i) ids = SOME (v,y)’
+      by (pop_assum mp_tac \\ rpt (pop_assum kall_tac)
+          \\ Induct_on ‘ids’ \\ fs[updateTheory.FIND_def]
+          \\ rpt strip_tac \\ Cases_on ‘h’ \\ fs[]
+          \\ Cases_on ‘x = q’ \\ fs[]
+          \\ cheat (*TODO: ids 1-1 *))
+    \\ fs[]
+    \\ ‘v = x’ by (cheat) \\ rveq
+    \\ TOP_CASE_TAC \\ fs[] \\ Cases_on ‘x’ \\ fs[] \\ rveq)
+   \\ ‘lookupCMLVar x ids = NONE’
+     by (CCONTR_TAC
+         \\ Cases_on ‘lookupCMLVar x ids’ \\ fs[] \\ Cases_on ‘x'’ \\ fs[])
+   \\ fs[] \\ rveq
+   \\ fs[ExpressionSemanticsTheory.eval_expr_cases, toFloVerEnv_def,
+         lookupFloVerVar_def, lookupCMLVar_def]
+   \\ (* id is fresh! *) cheat)
+  >- (
+   fs[] \\ rveq \\ Cases_on ‘op’ \\ fs[isFloVerExps_def]
+   >- (
+    rename1 ‘App (FP_uop uop) es’
+    \\ Cases_on ‘uop’ \\ fs[quantHeuristicsTheory.LIST_LENGTH_1] \\ rveq
+    \\ fs[toFloVerExp_def]
+    \\ drule isFloVerExps_toFloVerExp_succeeds \\ fs[]
+    \\ disch_then (qspecl_then [‘ids’, ‘freshId’] assume_tac) \\ fs[]
+    \\ fs[] \\ rveq \\ fs[ExpressionSemanticsTheory.eval_expr_cases]
+    \\ rveq
+    \\ rename1 ‘eval_expr (toFloVerEnv env ids) (λ e. SOME REAL) fexp v1 m1’
+    \\ ‘m1 = REAL’ by (Cases_on ‘m1’ \\ fs[MachineTypeTheory.isCompat_def])
+    \\ rveq \\ first_x_assum drule
+    \\ rpt (disch_then drule)
+    \\ disch_then assume_tac \\ fs[]
+    \\ imp_res_tac fpSemPropsTheory.evaluate_fp_opts_inv
+    \\ fs[toRealExp_def, terminationTheory.evaluate_def,
+          astTheory.getOpClass_def, semanticPrimitivesTheory.do_app_def,
+          realOpsTheory.real_uop_def, getRealUop_def,
+          ExpressionsTheory.evalUnop_def])
+   >- (
+    rename1 ‘App (FP_bop bop) es’
+    \\ Cases_on ‘bop’ \\ fs[quantHeuristicsTheory.LIST_LENGTH_2] \\ rveq
+    \\ fs[toFloVerExp_def]
+    \\ drule isFloVerExps_toFloVerExp_succeeds \\ fs[]
+    \\ disch_then (qspecl_then [‘e1’, ‘ids’, ‘freshId’] assume_tac) \\ fs[]
+    \\ fs[]
+    \\ rename1 ‘toFloVerExp ids freshId e1 = SOME (ids1, freshId1, fexp1)’
+    \\ drule isFloVerExps_toFloVerExp_succeeds \\ fs[]
+    \\ disch_then (qspecl_then [‘e2’, ‘ids1’, ‘freshId1’] assume_tac) \\ fs[]
+    \\ fs[] \\ rveq
+    \\ rename1 ‘eval_expr (toFloVerEnv env ids) (λ e. SOME REAL) (Binop (fpBopToFloVer _) fexp1 fexp2) r REAL’
+    \\ fs[ExpressionSemanticsTheory.eval_expr_cases]
+    \\ ‘m1 = REAL ∧ m2 = REAL’
+      by (Cases_on ‘m1’ \\ Cases_on ‘m2’
+          \\ fs[MachineTypeTheory.isJoin_def, MachineTypeTheory.isFixedPoint_def, MachineTypeTheory.join_fl_def] MachineTypeTheory.morePrecise_def, MachineTypeTheory.join_fl_def]
+
+Theorem FloverCmd_CakeML_real_imp:
+  ∀ e f r ids ids2 freshId st env st2.
+    isFloVerCmd e ∧
+    bstep f (toFloVerEnv env ids) (λ e. SOME REAL) r REAL ∧
+    toFloVerCmd ids freshId e = SOME(ids2, f) ⇒
+    evaluate st env [toRealExp e] = (st2, Rval [Real r])
+Proof
+  ho_match_mp_tac isFloVerCmd_ind \\ rpt strip_tac \\ fs[isFloVerCmd_def]
+  >- (
+   Cases_on ‘so’ \\ fs[toFloVerCmd_def]
+   \\ drule isFloVerExps_toFloVerExp_succeeds \\ fs[]
+   \\ disch_then (qspecl_then [‘ids’, ‘freshId’] assume_tac) \\ fs[] \\ fs[]
+   \\ drule isFloVerCmd_toFloVerCmd_succeeds \\ fs[]
+   \\ disch_then (qspecl_then [‘appendVar (Short x) freshId2 ids2'’, ‘freshId2 + 1’] assume_tac)
+   \\ fs[] \\ fs[] \\ rveq
+   \\ fs[bstep_cases]
+   \\ simp[toRealExp_def, terminationTheory.evaluate_def]
+
+ mp_tac (bstep_ind |> SPEC bstep_goal) \\ reverse impl_tac
+ >- (
+   rpt strip_tac \\ fs[] \\ rpt strip_tac \\ first_x_assum drule
+   \\ rpt (disch_then drule) \\ fs[])
+ \\ rpt strip_tac \\ fs[]
+
 Theorem CakeML_FloVer_real_equiv:
 ! e (st st2:'a semanticPrimitives$state) env e r.
   (* the CakeML code can be translated into FloVer input *)
@@ -19,31 +200,82 @@ Theorem CakeML_FloVer_real_equiv:
     toFloVerCmd [] 0 e = SOME (ids, f) /\
     (* evaluation on reals in CakeML is equivalent to evaluation in FloVer *)
     (evaluate st env [toRealExp e] = (st2, Rval [Real r]) <=>
-     bstep f (toFloVerEnv env ids) Gamma r REAL)
+     bstep f (toFloVerEnv env ids) (λ e. SOME M64) r REAL)
 Proof
-  cheat
+  rpt strip_tac
+  \\ imp_res_tac isFloVerCmd_toFloVerCmd_succeeds
+  \\ first_x_assum (qspecl_then [‘[]’, ‘0’] assume_tac) \\ fs[]
+  \\ EQ_TAC \\ rpt (pop_assum mp_tac)
 QED
+*)
 
+Definition env_rel_def:
+  env_rel env E (ids: ((string, string) id # num) list) =
+  (∀ (x:string) v w fp.
+   nsLookup env (Short x) = SOME v ∧
+    (v = Litv (Word64 w) ∨ v = FP_WordTree fp) ⇒
+    ∃ n r.
+    lookupCMLVar (Short x) ids = SOME (Short x,n) ∧
+    E n = SOME r ∧
+    case v of
+    | FP_WordTree fp => fp64_to_real (compress_word fp) = r
+    | Litv (Word64 w) => fp64_to_real w = r
+    | _ => F)
+End
+
+(*
 Theorem CakeML_FloVer_infer_error:
-! e (st st2:'a semanticPrimitives$state) env e w Gamma P analysisResult.
+  ∀ e (st st2:'a semanticPrimitives$state) env e Gamma P analysisResult.
   (* the CakeML code can be translated into FloVer input *)
-  isFloVerCmd e /\
-  (* the CakeML code returns a valid floating-point word *)
-  evaluate st env [e] = (st2, Rval [FP_WordTree w]) /\
+  isFloVerCmd e ∧
+  (* the free variables of the program are bound and sound with respect to P *)
+  (∀ x.
+   x IN vars e ⇒
+   nsLookup x = SOME v ∧
+   nsLookup x = SOME (Litv (Word64 w)) ⇒
+   fst (P x) ≤ fp64_to_real w ∧ fp64_to_real w ≤ snd (P x) ∧
+   nsLookup x = SOME (FP_WordTree fp) ⇒
+   fst (P x) ≤ fp64_to_real (compress_word fp) ∧ fp64_to_real (compress_word fp) ≤ snd (P x)) ∧
   (* translating to FloVer, running the pipeline succeeds *)
   getErrorbounds e Gamma P = SOME analysisResult ==>
-  ? ids f iv err r.
+  ? ids f iv err w r.
     (* the translation to FloVer does not fail *)
     toFloVerCmd [] 0 e = SOME (ids, f) /\
     (* the analysis result returned contains an error bound *)
     FloverMapTree_find (getRetExp f) analysisResult = SOME (iv,err) /\
     (* we can evaluate with a real-valued semantics *)
     evaluate st env [toRealExp e] = (st2, Rval [Real r]) /\
+    (* the CakeML code returns a valid floating-point word *)
+    evaluate st env [e] = (st2, Rval [FP_WordTree w]) /\
     (* the roundoff error is sound *)
     real$abs ((fp64_to_real (case (compress (FP_WordTree w)) of Litv (Word64 w) => w) - r))
       <= err
 Proof
-  cheat
+  rpt strip_tac
+  \\ imp_res_tac isFloVerCmd_toFloVerCmd_succeeds
+  \\ first_x_assum (qspecl_then [‘[]’, ‘0’] assume_tac)
+  \\ fsrw_tac [SATISFY_ss] [semanticPrimitivesTheory.compress_def]
+  \\ qpat_x_assum ‘getErrorbounds _ _ _ = _’ mp_tac
+  \\ simp[getErrorbounds_def]
+  \\ ntac 3 (TOP_CASE_TAC \\ fs[])
+  \\ rpt strip_tac \\ fs[] \\ rveq
+  \\ imp_res_tac CertificateCheckerTheory.CertificateCmd_checking_is_sound
+  \\ first_x_assum (qspec_then ‘freeVars f’ assume_tac) \\ fs[]
+  \\ ‘∃ E1. env_rel (env.v) E1 ids2’ by (cheat)
+  \\ first_x_assum (qspec_then ‘E1’ mp_tac)
+  \\ impl_tac
+  >- (
+   rpt strip_tac (* should follow from soundness of P for CakeML *)
+   \\ cheat)
+  \\ disch_then (qspec_then ‘E1’ assume_tac) \\ fs[]
+  \\ pop_assum mp_tac
+  \\ impl_tac
+  >- (
+   irule EnvironmentsTheory.approxEnv_refl \\ fs[]
+   \\ cheat)
+  \\ disch_then assume_tac \\ fs[]
+  \\ cheat
 QED
+*)
 
 val _ = export_theory ();
