icing/icingTestScript.sml
@@ -6,38 +6,28 @@ open compilerTheory basisFunctionsLib basisComputeLib basisProgTheory;
 (* FloVer *)
 open RealIntervalInferenceTheory ErrorIntervalInferenceTheory CertificateCheckerTheory;
 (* Icing *)
-open CakeMLtoFloVerTheory;
+open source_to_sourceTheory CakeMLtoFloVerTheory;
 (* HOL libs *)
 open machine_ieeeTheory binary_ieeeTheory realTheory realLib RealArith;
 open preamble;
 
 val _ = new_theory "icingTest";
 
-Definition doppler_hol_def:
-  doppler (u:word64, v:word64, t:word64) =
-  let
-  t1 = fp64_add roundTiesToEven (4644537666646730342w:word64)
-         (fp64_mul roundTiesToEven (4603579539098121011w:word64) t)
-  in
-  fp64_div roundTiesToEven
-  (fp64_mul roundTiesToEven
-   (fp64_negate t1)
-   v)
-  (fp64_mul roundTiesToEven
-   (fp64_add roundTiesToEven t1 u)
-   (fp64_add roundTiesToEven t1 u))
-End
+val _ = monadsyntax.enable_monadsyntax();
+val _ = monadsyntax.enable_monad "option";
 
 Definition doppler_cml_def:
   doppler_cml =
-  Dletrec
-    (Locs <|row := 2; col := 3; offset := 0|>
-     <|row := 7; col := 5; offset := 0|>)
+  Dletrec unknown_loc
     [("doppler","",
-      FpOptimise Opt
-      (Mat (Var (Short ""))
-        [(Pcon NONE [Pvar "u"; Pvar "v"; Pvar "t"],
-          Let (SOME "t1")
+      Fun "u" (Fun "v" (Fun "t"
+        (Let NONE
+         (App Opapp
+          [Var (Long "RuntimeProg" (Short "assert"));
+           (App Opapp
+            [App Opapp [Var (Short "="); Lit (IntLit 1)]; Lit (IntLit 1)])])
+         (FpOptimise Opt
+          (Let (SOME "t1")
             (App (FP_bop FP_Add)
               [
                 Lit (Word64 (4644537666646730342w:word64));
@@ -65,266 +55,96 @@ Definition doppler_cml_def:
                    Var (Short "u")])
                 ])
              ])
-           )]))]
+           ))))))]
 End
 
-Theorem doppler_opt =
-  EVAL ``HD (source_to_source$compile_decs
+Definition doppler_opt_def:
+  doppler_opt =
+  HD (source_to_source$compile_decs
            <| optimisations := [
                (Binop FP_Mul (Var 0) (Binop FP_Add (Var 1) (Var 2)),
                 Terop FP_Fma (Var 0) (Var 1) (Var 2))];
                canOpt := T |>
-           [doppler_cml])``;
+           [doppler_cml])
+End
+
+Definition getFunctions_def:
+  getFunctions (Dletrec l funs) = SOME funs ∧
+  getFunctions _ = NONE
+End
 
 Definition doppler_body_def:
-  doppler_body =
-    case doppler_cml of
-    | Dletrec _ [ (_, _, e)] => e
+doppler_body = getFunctions doppler_cml
+End
+
+Definition doppler_opt_body_def:
+doppler_opt_body = getFunctions doppler_opt
+End
+
+Definition strip_funs_def:
+  strip_funs (Fun var body) =
+    (let (vars, body) = strip_funs body in
+    (var :: vars, body)) ∧
+  strip_funs e = ([], e)
+End
+
+Definition strip_assert_def:
+  strip_assert (Let NONE P body) =
+    (case P of
+    | App op [fN; P] =>
+      if (op = Opapp ∧ fN = Var (Long "RuntimeProg" (Short "assert")))
+      then SOME (P, body)
+      else NONE
+    | _ => NONE) ∧
+  strip_assert _ = NONE
+End
+
+Definition strip_noopt_def:
+  strip_noopt (FpOptimise NoOpt e) = e ∧
+  strip_noopt e = e
+End
+
+Definition prepare_kernel_def:
+  prepare_kernel exps =
+    case exps of
+    | NONE => NONE
+    | SOME exps =>
+      if (LENGTH exps ≠ 1)
+      then NONE
+      else
+        case exps of
+        | [(n1, n2, e)] =>
+        let
+          fN = strip_noopt e;
+          (vars, body) = strip_funs fN in
+        do
+          (P, body) <- strip_assert body;
+          (* FIXME: should not need to strip noopt annotations here *)
+          return (vars, P, strip_noopt body);
+        od
+        | _ => NONE
 End
 
 Definition optimised_doppler_body_def:
-  optimised_doppler_body =
-    case (^(rhs (concl doppler_opt))) of
-    | Dletrec _ [ (_, _, e)] => e
+  optimised_doppler_body = prepare_kernel doppler_opt_body
 End
 
-(*
-Definition isMorePrecise_def:
-  isMorePrecise f1 f2 Gamma P =
-  let
-    floverF1 = THE (toFloVerCmd [] 0 (rm_top_match (strip f1)));
-    floverF2 = THE (toFloVerCmd [] 0 (rm_top_match (strip f2)));
-    errsF1 = THE (getErrorbounds f1 Gamma P);
-    errsF2 = THE (getErrorbounds f2 Gamma P);
-  in
-    case FloverMapTree_find (getRetExp floverF1) errsF1 of
-    | NONE => F
-    | SOME (iv1, err1) =>
-    (case FloverMapTree_find (getRetExp floverF2) errsF2 of
-    | NONE => F
-    | SOME (iv2, err2) => (err2:real <= err1))
+Definition Gamma_def:
+  Gamma =
+    let (vars, varMap, freshId) = prepareVars (FST (THE optimised_doppler_body)) in
+      prepareGamma vars
 End
-*)
 
-val Gamma = EVAL ``FloverMapTree_insert (Var 0) M64 (
-FloverMapTree_insert (Var 1) M64 (
-FloverMapTree_insert (Var 2) M64 (
-FloverMapTree_insert (Var 3) M64 (
-FloverMapTree_insert (Var 4) M64 (
-FloverMapTree_insert (Var 5) M64 FloverMapTree_empty)))))``;
+val P = ``λ x:num. (0,100):(real#real)``;
 
-val P = ``λ x:num. (1,2):(real#real)``;
+val _ = computeLib.del_funs [sptreeTheory.subspt_def];
+
+val _ = computeLib.add_funs [realTheory.REAL_INV_1OVER, binary_ieeeTheory.float_to_real_def, sptreeTheory.subspt_eq, sptreeTheory.lookup_def];
 
 val test =
 EVAL (Parse.Term `
       getErrorbounds
-      optimised_doppler_body
-      ^(rhs (concl Gamma))
+      (THE optimised_doppler_body)
       ^P`);
 
-(*
-val test2 =
-EVAL (Parse.Term `
-      isMorePrecise
-      doppler_body
-      optimised_doppler_body
-      ^(rhs (concl Gamma))
-      ^P`)
-*)
-val _ = computeLib.add_funs [realTheory.REAL_INV_1OVER, binary_ieeeTheory.float_to_real_def];
-
-val doppler_def = EVAL ``
-(THE (toFloVerCmd [] 0 (rm_top_match (strip optimised_doppler_body))))``
-
-val real_iv_bounds = EVAL ``inferIntervalboundsCmd
-(SND (THE (toFloVerCmd [] 0 (rm_top_match (strip optimised_doppler_body)))))
-(λ x. (1,2)) FloverMapTree_empty``;
-
-val typeMap = EVAL (Parse.Term `case (TypeValidator$getValidMapCmd  ^(rhs (concl Gamma))
-(SND (THE (toFloVerCmd [] 0 (rm_top_match (strip optimised_doppler_body)))))
-FloverMapTree_empty) of Succes t => t`);
-
-val error_bounds = curry save_thm "error_bounds_thm" (EVAL (Parse.Term `inferErrorboundCmd
-(SND (THE (toFloVerCmd [] 0 (rm_top_match (strip optimised_doppler_body)))))
-^(rhs (concl typeMap))
-(THE (^(rhs (concl real_iv_bounds))))
-FloverMapTree_empty`));
-
-(* The "additional"/meta-theorem theorem:
-Theorem optimised_doppler_more_accuracte:
-  error (optimised_doppler) ≤ error (doppler_cml)
-Proof
-  (* TODO *)
-  cheat
-QED
- *)
-
 val _ = export_theory();
-
-(** FAILED ATTEMPTS below
-
-Definition strip_noopt_def:
-  strip_noopt (Lit l) = Lit l /\
-  strip_noopt (Var x) = Var x /\
-  strip_noopt (Raise e) =
-    Raise (strip_noopt e) /\
-  strip_noopt (Handle e pes) =
-    Handle (strip_noopt e) (MAP (\ (p,e). (p, strip_noopt e)) pes) /\
-  strip_noopt (Con mod exps) =
-    Con mod (MAP strip_noopt exps) ∧
-  strip_noopt (Fun s e) =
-    Fun s (strip_noopt e) /\
-  strip_noopt (ast$App op exps) =
-    (App op (MAP strip_noopt exps)) /\
-  strip_noopt (Log lop e2 e3) =
-    Log lop (strip_noopt e2) (strip_noopt e3) /\
-  strip_noopt (If e1 e2 e3) =
-    If (strip_noopt e1) (strip_noopt e2) (strip_noopt e3) /\
-  strip_noopt (Mat e pes) =
-    Mat (strip_noopt e) (MAP (\ (p,e). (p, strip_noopt e)) pes) /\
-  strip_noopt (Let so e1 e2) =
-    Let so (strip_noopt e1) (strip_noopt e2) /\
-  strip_noopt (Letrec ses e) =
-    Letrec (MAP (\ (s1,s2,e). (s1, s2, strip_noopt e)) ses) (strip_noopt e) /\
-  strip_noopt (Tannot e t) =
-    Tannot (strip_noopt e) t /\
-  strip_noopt (Lannot e l) =
-    Lannot (strip_noopt e) l /\
-  strip_noopt (FpOptimise NoOpt e) =
-    (strip_noopt e) ∧
-  strip_noopt (FpOptimise sc e) =
-    FpOptimise sc (strip_noopt e)
-Termination
-  WF_REL_TAC `measure exp_size` \\ fs[]
-  \\ rpt conj_tac
-  >- (Induct_on `ses` \\ fs[astTheory.exp_size_def]
-      \\ rpt strip_tac \\ res_tac \\ rveq \\ fs[astTheory.exp_size_def]
-      \\ first_x_assum (qspec_then `e` assume_tac) \\ fs[])
-  >- (Induct_on `pes` \\ fs[astTheory.exp_size_def]
-      \\ rpt strip_tac \\ res_tac \\ rveq \\ fs[astTheory.exp_size_def]
-      \\ first_x_assum (qspec_then `e` assume_tac) \\ fs[])
-  >- (Induct_on `pes` \\ fs[astTheory.exp_size_def]
-      \\ rpt strip_tac \\ res_tac \\ rveq \\ fs[astTheory.exp_size_def]
-      \\ first_x_assum (qspec_then `e` assume_tac) \\ fs[])
-  >- (Induct_on `exps` \\ fs[astTheory.exp_size_def]
-      \\ rpt strip_tac \\ res_tac \\ rveq \\ fs[astTheory.exp_size_def]
-      \\ first_x_assum (qspec_then `op` assume_tac) \\ fs[])
-  >- (Induct_on `exps` \\ fs[astTheory.exp_size_def]
-      \\ rpt strip_tac \\ res_tac \\ rveq \\ fs[astTheory.exp_size_def]
-      \\ first_x_assum (qspec_then `mod'` assume_tac) \\ fs[])
-End
-
-Definition strip_noopt_exps_def:
-  strip_noopt_exps [] = [] ∧
-  strip_noopt_exps [e] = [strip_noopt e] ∧
-  strip_noopt_exps (e1::es) = (strip_noopt_exps [e1]) ++ (strip_noopt_exps es)
-End
-
-Definition strip_noopt_decs_def:
-  strip_noopt_decs [] = [] /\
-  strip_noopt_decs [Dlet l p e] = [Dlet l p (HD (strip_noopt_exps [e]))] /\
-  strip_noopt_decs [Dletrec ls vexps] =
-    [Dletrec ls (MAP (\ (v1,v2,e). (v1,v2,HD (strip_noopt_exps [e]))) vexps)] /\
-  strip_noopt_decs [Dtype l t] = [Dtype l t] /\
-  strip_noopt_decs [Dtabbrev l vars t ast] = [Dtabbrev l vars t ast] /\
-  strip_noopt_decs [Dexn l c asts] = [Dexn l c asts] /\
-  strip_noopt_decs [Dmod m decls] = [Dmod m (strip_noopt_decs decls)] /\
-  strip_noopt_decs [Dlocal decls1 decls2] =
-    [Dlocal (strip_noopt_decs decls1) (strip_noopt_decs decls2)] /\
-  strip_noopt_decs (d1::d2::ds) = strip_noopt_decs [d1] ++ strip_noopt_decs (d2::ds)
-Termination
-  wf_rel_tac `measure dec1_size`
-End
-
-val cml_thm = translate doppler_def;
-val cml_def = fetch "-" "doppler_v_def";
-
-EVAL “rewriteFPexp [fp_comm_gen FP_Add] (App (FP_bop FP_Add) [Var (Short "t1"); Var (Short "t2")])”
-                    (Binop FP_Mul (Var 0) (Binop FP_Add (Var 1) (Var 2)),
-                      Terop FP_Fma (Var 0) (Var 1) (Var 2))] ”
-
-val cml_opt = let val theDef = rhs (concl cml_def); in EVAL (Parse.Term `strip_noopt_decs ^theDef`) end;
-
-
-Theorem extend_dec_ienv_empty:
-   !ienv.
-    extend_dec_ienv ienv <| inf_v := nsEmpty; inf_c := nsEmpty; inf_t := nsEmpty |> = ienv ∧
-    extend_dec_ienv <| inf_v := nsEmpty; inf_c := nsEmpty; inf_t := nsEmpty |> ienv = ienv
-Proof
-  rw [extend_dec_ienv_def, inf_env_component_equality]
-QED
-
-Theorem nsAppend_assoc:
-nsAppend (nsAppend A B) C = nsAppend A (nsAppend B C)
-Proof
- Cases_on `A` \\ Cases_on `B` \\ Cases_on `C` \\ fs[namespaceTheory.nsAppend_def]
-QED
-
-Theorem infer_ds_split:
- ∀ prog1 prog2 conf1 state.
-   infer_ds conf1 (prog1 ++ prog2) state =
-   case (infer_ds conf1 prog1 state) of
-   | (infer$Success ienv1, state2) =>
-     (case infer_ds (extend_dec_ienv ienv1 conf1) prog2 state2 of
-     | (infer$Success ienv2, state3) => (infer$Success (extend_dec_ienv ienv2 ienv1), state3)
-     | res => res)
-   | res => res
-Proof
-  Induct_on `prog1`  \\ rpt strip_tac \\ fs[]
-  >- (
-   fs [infer_d_def, st_ex_return_def, extend_dec_ienv_empty] \\ rpt (TOP_CASE_TAC \\ fs[]))
-  \\ simp[infer_d_def, st_ex_return_def, st_ex_bind_def, extend_dec_ienv_empty]
-  \\ rename1 `infer_d conf1 h state1`
-  \\ Cases_on `infer_d conf1 h state1` \\ fs[]
-  \\ Cases_on `q` \\ fs[]
-  \\ rename1 `infer_ds (extend_dec_ienv conf2 conf1) prog1 r`
-  \\ Cases_on `infer_ds (extend_dec_ienv conf2 conf1) prog1 r` \\ fs[]
-  \\ Cases_on `q` \\ fs[extend_dec_ienv_def, Once nsAppend_assoc]
-  \\ qmatch_goalsub_abbrev_tac `infer_ds ienv3 prog2 r'`
-  \\ Cases_on `infer_ds ienv3 prog2 r'` \\ fs[]
-  \\ Cases_on `q` \\ fs[]
-QED
-
-SIMP_RULE std_ss [infer_ds_split] (GEN_ALL (Q.SPECL [`ienv`, `prog1 ++ prog2`] infertype_prog_def));
-(*
-val theEnv = rand (rhs (concl (basisTypeCheckTheory.basis_types)));
-
-  EVAL  (Parse.Term `infertype_prog (^theEnv) (^doppler_cml)`);
-
-val dopper_opt =
-  EVAL (Parse.Term `source_to_source$compile_decs <| optimisations:= [fp_comm_gen FP_Add]; canOpt := T |> ^doppler_cml`)
-
-
-val doppler_cml =
-  ``"fun doppler (u:Word64.word, v:Word64.word, t:Word64.word) = let val t1 = Double.+ (Double.fromString \"331.4\") (Double.* (Double.fromString \"0.6\") t); in Double./ (Double.* (Double.~ t1) v) (Double.* (Double.+ t1 u) (Double.+ t1 u)) end"``;
-
-Definition test_def:
-  test x = fp64_add roundTiesToEven x x
-End
-
-val r = translate test_def;
-
-val simple_fun =
-  ``"fun f () = print \"Hello\";"``;
-
-val [empty_ffi] = decls "empty_ffi";
-val _ = computeLib.monitoring := SOME (same_const empty_ffi);
-
-val cmp = wordsLib.words_compset ()
-val () = computeLib.extend_compset
-    [computeLib.Extenders
-      [inferenceComputeLib.add_inference_compset,
-      basicComputeLib.add_basic_compset
-      ],
-     computeLib.Defs
-      [basisProgTheory.basis_def
-      ],
-    computeLib.Tys
-    [    ]
-    ] cmp
-val inf_eval = computeLib.CBV_CONV cmp
-
-val test = EVAL (Parse.Term `compile_icing basis init_config source_to_source$no_fp_opt_conf (^doppler_cml)`);
-EVAL (Parse.term `infertype_prog
-*)
-*)
